outlined complicated compiler case

src/Pyrosome/Lang/Multilanguages.v
@@ -27,233 +27,6 @@ From Pyrosome Require Import Compilers.Compilers Elab.ElabCompilers.
 Import CompilerDefs.Notations. (* for `match # from high_level_multilanguage with` *)
 (* CompilerDefs, for preserving_compiler_ext, is already imported. Prolly through something else. *)
 
-(* The polymorphic languages *)
-(* NOTE: the following is abstracted from the definition of stlc_parameterized in PolyCompilers.v *)
-Definition parameterize_wrapper (l : lang) : lang := 
-    let ps := (elab_param "D" (l
-                                 ++ exp_ret 
-                                 ++ exp_subst_base
-                                 ++ value_subst
-                                 )
-               [("sub", Some 2);
-                ("ty", Some 0);
-                ("env", Some 0);
-                ("val",Some 2);
-                ("exp",Some 2)]) in
-  parameterize_lang "D" {{s #"ty_env"}}
-    ps l.
-
-Local Definition evp'_general (l : lang) : lang := 
-    let ps := (elab_param "D" (l ++ exp_ret ++ exp_subst_base
-                                 ++ value_subst)
-               [("sub", Some 2);
-                ("ty", Some 0);
-                ("env", Some 0);
-                ("val",Some 2);
-                ("exp",Some 2)]) in
-  parameterize_lang "D" {{s #"ty_env"}}
-    ps (exp_ret ++ exp_subst_base ++ value_subst).
-
-Ltac solve_parameterize_wrapper l := (* comments are copied over from PolyCompilers.v*)
-  change (exp_parameterized++val_parameterized) with (evp'_general l);
-  (*TODO: phrase exp_and_val_parameterized as parameterized in definition*)
-  (*TODO: need to strengthen parameterization pl w/ add'l language?
-    Currently cheating.
-   *)
-  eapply parameterize_lang_preserving_ext;
-    try typeclasses eauto;
-    [repeat t';  constructor (*TODO: include in t'*)
-    | now prove_from_known_elabs..
-    | vm_compute; exact I].
-
-Definition typed_bool_parameterized' := parameterize_wrapper typed_bool. 
-
-Lemma typed_bool_parameterized'_wf
-  : wf_lang_ext ((exp_parameterized ++ val_parameterized) ++ ty_env_lang)
-      typed_bool_parameterized'.
-Proof. solve_parameterize_wrapper typed_bool. Qed. 
-#[export] Hint Resolve typed_bool_parameterized'_wf : elab_pfs.
-
-Definition typed_bool_parameterized_def : lang :=
-{[l
-    [:= "D" : #"ty_env",
-        "D'" : #"ty_env",
-        "g" : #"ty_sub" "D" "D'"
-        ----------------------------------------------- ("ty_subst bool")
-        #"ty_subst" "g" #"bool" = 
-        #"bool"
-        : #"ty" "D"
-    ]
-]}.
-Derive typed_bool_parameterized
-  SuchThat (elab_lang_ext (typed_bool_parameterized' ++
-                                exp_param_substs ++
-                                exp_ty_subst ++
-                                val_param_substs ++
-                                val_ty_subst ++
-                                env_ty_subst ++
-                                ty_subst_lang ++
-                                exp_parameterized ++ val_parameterized ++ ty_env_lang
-                                )
-              typed_bool_parameterized_def typed_bool_parameterized)
-  As typed_bool_wf.
-Proof. auto_elab.
-Qed. 
-#[export] Hint Resolve typed_bool_wf : elab_pfs.
-
-Definition usubst_parameterized' := parameterize_wrapper usubst. 
-
-Lemma usubst_parameterized'_wf
-  : wf_lang_ext ((exp_parameterized ++ val_parameterized) ++ ty_env_lang)
-      usubst_parameterized'.
-Proof. solve_parameterize_wrapper usubst. Qed.
-#[export] Hint Resolve usubst_parameterized'_wf : elab_pfs.
-
-Definition usubst_parameterized_def : lang :=
-{[l
-    [:= "D" : #"ty_env",
-        "D'" : #"ty_env",
-        "g" : #"ty_sub" "D" "D'"
-        ----------------------------------------------- ("ty_subst star")
-        #"ty_subst" "g" #"*" = 
-        #"*"
-        : #"ty" "D"
-    ]
-]}.
-Derive usubst_parameterized
-  SuchThat (elab_lang_ext (usubst_parameterized' ++
-                                exp_param_substs ++
-                                exp_ty_subst ++
-                                val_param_substs ++
-                                val_ty_subst ++
-                                env_ty_subst ++
-                                ty_subst_lang ++
-                                exp_parameterized ++ val_parameterized ++ ty_env_lang
-                                )
-              usubst_parameterized_def usubst_parameterized)
-  As usubst_parameterized_wf.
-Proof. auto_elab.
-Qed. 
-#[export] Hint Resolve usubst_parameterized_wf : elab_pfs.
-
-Definition stlc_poly_def : lang :=
-{[l
-    [:= "D" : #"ty_env",
-        "D'" : #"ty_env",
-        "d" : #"ty_sub" "D" "D'",
-        "A" : #"ty" "D'",
-        "B" : #"ty" "D'"
-        ----------------------------------------------- ("ty_subst-arrow dist")
-        #"ty_subst" "d" (#"->" "A" "B") = 
-        #"->" (#"ty_subst" "d" "A") (#"ty_subst" "d" "B")
-        : #"ty" "D"
-    ]
-]}.
-Derive stlc_poly
-  SuchThat (elab_lang_ext (stlc_parameterized ++
-                                exp_param_substs ++
-                                exp_ty_subst ++
-                                val_param_substs ++
-                                val_ty_subst ++
-                                env_ty_subst ++
-                                ty_subst_lang ++
-                                exp_parameterized ++ val_parameterized ++ ty_env_lang
-                                )
-              stlc_poly_def stlc_poly)
-  As stlc_poly_wf.
-Proof. auto_elab. (* QUESTION FOR DUSTIN: WHY? *)
-Qed. 
-#[export] Hint Resolve stlc_poly_wf : elab_pfs.
-
-
-Definition utlc_parameterized := 
-    let ps := (elab_param "D" (utlc ++ usubst ++ exp_ret ++ exp_subst_base
-                                 ++ value_subst)
-               [("sub", Some 2);
-                ("ty", Some 0);
-                ("env", Some 0);
-                ("val",Some 2);
-                ("exp",Some 2)]) in
-  parameterize_lang "D" {{s #"ty_env"}}
-    ps utlc.
-
-Local Definition evp'_utlc : lang := 
-    let ps := (elab_param "D" (utlc ++ usubst ++ exp_ret ++ exp_subst_base
-                                 ++ value_subst)
-               [("sub", Some 2);
-                ("ty", Some 0);
-                ("env", Some 0);
-                ("val",Some 2);
-                ("exp",Some 2)]) in
-  parameterize_lang "D" {{s #"ty_env"}}
-    ps (usubst ++ exp_ret ++ exp_subst_base ++ value_subst).
-
-
-(* NOTE: is this ok? *)
-(* NOT IMMMEDIATELY RELEVANT *)
-(* BOTH UTLC_P AND UNTYPED_BOOL_P *)
-Lemma utlc_parameterized_wf
-  : wf_lang_ext ((usubst_parameterized' ++ exp_parameterized ++ val_parameterized) ++ ty_env_lang)
-      utlc_parameterized.
-Proof. 
-  replace (usubst_parameterized' ++ exp_parameterized ++ val_parameterized) with evp'_utlc.
-  - eapply parameterize_lang_preserving_ext;
-    try typeclasses eauto;
-    [repeat t';  constructor (*TODO: include in t'*)
-    | now prove_from_known_elabs..
-    | vm_compute; exact I].
-  - cbv; reflexivity. 
-Qed. 
-#[export] Hint Resolve utlc_parameterized_wf : elab_pfs.
-
-Definition untyped_bool_parameterized := 
-    let ps := (elab_param "D" (untyped_bool ++ usubst ++ exp_ret ++ exp_subst_base
-                                 ++ value_subst)
-               [("sub", Some 2);
-                ("ty", Some 0);
-                ("env", Some 0);
-                ("val",Some 2);
-                ("exp",Some 2)]) in
-  parameterize_lang "D" {{s #"ty_env"}}
-    ps untyped_bool.
-
-Local Definition evp'_untyped_bool : lang := 
-    let ps := (elab_param "D" (untyped_bool ++ usubst ++ exp_ret ++ exp_subst_base
-                                 ++ value_subst)
-               [("sub", Some 2);
-                ("ty", Some 0);
-                ("env", Some 0);
-                ("val",Some 2);
-                ("exp",Some 2)]) in
-  parameterize_lang "D" {{s #"ty_env"}}
-    ps (usubst ++ exp_ret ++ exp_subst_base ++ value_subst).
-
-Lemma untyped_bool_parameterized_wf
-  : wf_lang_ext ((usubst_parameterized' ++ exp_parameterized ++ val_parameterized) ++ ty_env_lang)
-      untyped_bool_parameterized.
-Proof. 
-  replace (usubst_parameterized' ++ exp_parameterized ++ val_parameterized) with evp'_untyped_bool.
-  - eapply parameterize_lang_preserving_ext;
-    try typeclasses eauto;
-    [repeat t';  constructor (*TODO: include in t'*)
-    | now prove_from_known_elabs..
-    | vm_compute; exact I].
-  - cbv; reflexivity. 
-Qed. 
-#[export] Hint Resolve utlc_parameterized_wf : elab_pfs.
-
-
-
-(* 
-TODO: 
-- typerec func (DONE)
-- ty_subst (DONE)
-- convoy for simple to poly compiler
-- parameterize boundaries (* STARTED, not done *)
-- remaining langs parameterized (ultc_bool, mif, uif, boolhuh)
-- convoy for poly to poly compiler
-*)
-
 Definition boundaries_def : lang :=
   {[l/subst [exp_subst++value_subst] 
     [:| "G" : #"env",
@@ -350,6 +123,656 @@ Derive boundaries
         As boundaries_wf.
 Proof. auto_elab. Qed.
 #[export] Hint Resolve boundaries_wf : elab_pfs.
+
+
+(* NOTE: the following is abstracted from the definition of stlc_parameterized in PolyCompilers.v *)
+Definition parameterize_wrapper (l : lang) : lang := 
+    let ps := (elab_param "D" (l
+                                 ++ exp_ret 
+                                 ++ exp_subst_base
+                                 ++ value_subst
+                                 )
+               [("sub", Some 2);
+                ("ty", Some 0);
+                ("env", Some 0);
+                ("val",Some 2);
+                ("exp",Some 2)]) in
+  parameterize_lang "D" {{s #"ty_env"}}
+    ps l.
+
+Local Definition evp'_general (l : lang) : lang := 
+    let ps := (elab_param "D" (l ++ exp_ret ++ exp_subst_base
+                                 ++ value_subst)
+               [("sub", Some 2);
+                ("ty", Some 0);
+                ("env", Some 0);
+                ("val",Some 2);
+                ("exp",Some 2)]) in
+  parameterize_lang "D" {{s #"ty_env"}}
+    ps (exp_ret ++ exp_subst_base ++ value_subst).
+
+Ltac solve_parameterize_wrapper l := (* comments are copied over from PolyCompilers.v*)
+  change (exp_parameterized++val_parameterized) with (evp'_general l);
+  (*TODO: phrase exp_and_val_parameterized as parameterized in definition*)
+  (*TODO: need to strengthen parameterization pl w/ add'l language?
+    Currently cheating.
+   *)
+  eapply parameterize_lang_preserving_ext;
+    try typeclasses eauto;
+    [repeat t';  constructor (*TODO: include in t'*)
+    | now prove_from_known_elabs..
+    | vm_compute; exact I].
+
+Definition typed_bool_parameterized := parameterize_wrapper typed_bool. 
+
+Lemma typed_bool_parameterized_wf
+  : wf_lang_ext ((exp_parameterized ++ val_parameterized) ++ ty_env_lang)
+      typed_bool_parameterized.
+Proof. solve_parameterize_wrapper typed_bool. Qed. 
+#[export] Hint Resolve typed_bool_parameterized_wf : elab_pfs.
+
+Definition typed_bool_ty_subst_def : lang :=
+{[l
+    [:= "D" : #"ty_env",
+        "D'" : #"ty_env",
+        "g" : #"ty_sub" "D" "D'"
+        ----------------------------------------------- ("ty_subst bool")
+        #"ty_subst" "g" #"bool" = 
+        #"bool"
+        : #"ty" "D"
+    ]
+]}.
+Derive typed_bool_ty_subst
+  SuchThat (elab_lang_ext (typed_bool_parameterized ++
+                                exp_param_substs ++
+                                exp_ty_subst ++
+                                val_param_substs ++
+                                val_ty_subst ++
+                                env_ty_subst ++
+                                ty_subst_lang ++
+                                exp_parameterized ++ val_parameterized ++ ty_env_lang
+                                )
+              typed_bool_ty_subst_def typed_bool_ty_subst)
+  As typed_bool_ty_subst_wf.
+Proof. auto_elab.
+Qed. 
+#[export] Hint Resolve typed_bool_ty_subst_wf : elab_pfs.
+
+Definition usubst_parameterized := parameterize_wrapper usubst. 
+
+Lemma usubst_parameterized_wf
+  : wf_lang_ext ((exp_parameterized ++ val_parameterized) ++ ty_env_lang)
+      usubst_parameterized.
+Proof. solve_parameterize_wrapper usubst. Qed.
+#[export] Hint Resolve usubst_parameterized_wf : elab_pfs.
+
+Definition usubst_ty_subst_def : lang :=
+{[l
+    [:= "D" : #"ty_env",
+        "D'" : #"ty_env",
+        "g" : #"ty_sub" "D" "D'"
+        ----------------------------------------------- ("ty_subst star")
+        #"ty_subst" "g" #"*" = 
+        #"*"
+        : #"ty" "D"
+    ]
+]}.
+Derive usubst_ty_subst
+  SuchThat (elab_lang_ext (usubst_parameterized ++
+                                exp_param_substs ++
+                                exp_ty_subst ++
+                                val_param_substs ++
+                                val_ty_subst ++
+                                env_ty_subst ++
+                                ty_subst_lang ++
+                                exp_parameterized ++ val_parameterized ++ ty_env_lang
+                                )
+              usubst_ty_subst_def usubst_ty_subst)
+  As usubst_ty_subst_wf.
+Proof. auto_elab.
+Qed. 
+#[export] Hint Resolve usubst_ty_subst_wf : elab_pfs.
+
+Definition stlc_ty_subst_def : lang :=
+{[l
+    [:= "D" : #"ty_env",
+        "D'" : #"ty_env",
+        "d" : #"ty_sub" "D" "D'",
+        "A" : #"ty" "D'",
+        "B" : #"ty" "D'"
+        ----------------------------------------------- ("ty_subst-arrow dist")
+        #"ty_subst" "d" (#"->" "A" "B") = 
+        #"->" (#"ty_subst" "d" "A") (#"ty_subst" "d" "B")
+        : #"ty" "D"
+    ]
+]}.
+Derive stlc_ty_subst
+  SuchThat (elab_lang_ext (stlc_parameterized ++
+                                exp_param_substs ++
+                                exp_ty_subst ++
+                                val_param_substs ++
+                                val_ty_subst ++
+                                env_ty_subst ++
+                                ty_subst_lang ++
+                                exp_parameterized ++ val_parameterized ++ ty_env_lang
+                                )
+              stlc_ty_subst_def stlc_ty_subst)
+  As stlc_ty_subst_wf.
+Proof. auto_elab. (* QUESTION FOR DUSTIN: WHY? *)
+Qed. 
+#[export] Hint Resolve stlc_ty_subst_wf : elab_pfs.
+
+Fixpoint ty_wkn_n n :=
+  match n with
+  | 0 => {{e #"ty_id"}}
+  | 1 => {{e #"ty_wkn"}}
+  | S n' => {{e #"ty_cmp" #"ty_wkn" {ty_wkn_n n'} }}
+  end.
+
+Definition ty_ovar n :=
+  match n with 
+  | 0 => {{e #"ty_hd"}} (* bc ty_subst ty_id ty_hd is just ty_hd *)
+  | S _ => {{e #"ty_subst" {ty_wkn_n n} #"ty_hd" }}
+  end.  
+
+Definition A_var := {{e #"ty_subst" (#"ty_snoc" (#"ty_cmp" #"ty_wkn" (#"ty_snoc" #"ty_id" "t1")) #"ty_hd") (#"->" (#"ty_subst" (#"ty_snoc" {ty_wkn_n 2} {ty_ovar 0}) "sigma") (#"ty_subst" (#"ty_snoc" {ty_wkn_n 2} (#"->" {ty_ovar 1} {ty_ovar 0})) "sigma")) }}.
+
+Definition type_casing_def : lang :=
+  {[l
+    [:| "D" : #"ty_env",
+        "G" : #"env" "D",
+        "mu" : #"ty" "D", (* is mu *)
+        "sigma" : #"ty" (#"ty_ext" "D"), (* this is sigma. it has a variable (hence the ext *)
+        "e1" : #"exp" "D" "G" (#"ty_subst" (#"ty_snoc" #"ty_id" #"*") "sigma"), (* substitute identity type for all except the last (which is A), which we change to star *)
+        "e2" : #"exp" "D" "G" (#"ty_subst" (#"ty_snoc" #"ty_id" #"bool") "sigma"),
+        "e3" : #"exp" "D" "G" (#"All" (#"->" "sigma" (#"All" (#"->" (#"ty_subst" (#"ty_snoc" {ty_wkn_n 2} {ty_ovar 0}) "sigma") (#"ty_subst" (#"ty_snoc" {ty_wkn_n 2} (#"->" {ty_ovar 1} {ty_ovar 0})) "sigma"))))) (* look at arrow case in 134 *)
+        -----------------------------------------------
+        #"typerec" "mu" "sigma" "e1" "e2" "e3"
+        : #"exp" "D" "G" (#"ty_subst" (#"ty_snoc" #"ty_id" "mu") "sigma") (* verbose way of writing the [u/t]sigma in the rule on 134, verbose in that its the _full_ substitution *)
+    ];
+    [:= "D" : #"ty_env",
+        "G" : #"env" "D",
+        "sigma" : #"ty" (#"ty_ext" "D"),
+        "e1" : #"exp" "D" "G" (#"ty_subst" (#"ty_snoc" #"ty_id" #"*") "sigma"),
+        "e2" : #"exp" "D" "G" (#"ty_subst" (#"ty_snoc" #"ty_id" #"bool") "sigma"),
+        "e3" : #"exp" "D" "G" (#"All" (#"->" "sigma" (#"All" (#"->" (#"ty_subst" (#"ty_snoc" {ty_wkn_n 2} {ty_ovar 0}) "sigma") (#"ty_subst" (#"ty_snoc" {ty_wkn_n 2} (#"->" {ty_ovar 1} {ty_ovar 0})) "sigma")))))
+        ----------------------------------------------- ("typerec star")
+        #"typerec" #"*" "sigma" "e1" "e2" "e3"  
+        = "e1" : #"exp" "D" "G" (#"ty_subst" (#"ty_snoc" #"ty_id" #"*") "sigma")
+    ];
+    [:= "D" : #"ty_env",
+        "G" : #"env" "D",
+        "sigma" : #"ty" (#"ty_ext" "D"),
+        "e1" : #"exp" "D" "G" (#"ty_subst" (#"ty_snoc" #"ty_id" #"*") "sigma"),
+        "e2" : #"exp" "D" "G" (#"ty_subst" (#"ty_snoc" #"ty_id" #"bool") "sigma"),
+        "e3" : #"exp" "D" "G" (#"All" (#"->" "sigma" (#"All" (#"->" (#"ty_subst" (#"ty_snoc" {ty_wkn_n 2} {ty_ovar 0}) "sigma") (#"ty_subst" (#"ty_snoc" {ty_wkn_n 2} (#"->" {ty_ovar 1} {ty_ovar 0})) "sigma")))))
+        ----------------------------------------------- ("typerec bool")
+        #"typerec" #"bool" "sigma" "e1" "e2" "e3"  
+        = "e2" : #"exp" "D" "G" (#"ty_subst" (#"ty_snoc" #"ty_id" #"bool") "sigma")
+    ];
+    [:= "D" : #"ty_env",
+        "G" : #"env" "D",
+        "sigma" : #"ty" (#"ty_ext" "D"),
+        "t1" : #"ty" "D",
+        "t2" : #"ty" "D",
+        "e1" : #"exp" "D" "G" (#"ty_subst" (#"ty_snoc" #"ty_id" #"*") "sigma"),
+        "e2" : #"exp" "D" "G" (#"ty_subst" (#"ty_snoc" #"ty_id" #"bool") "sigma"),
+        "e3" : #"exp" "D" "G" (#"All" (#"->" "sigma" (#"All" (#"->" (#"ty_subst" (#"ty_snoc" {ty_wkn_n 2} {ty_ovar 0}) "sigma") (#"ty_subst" (#"ty_snoc" {ty_wkn_n 2} (#"->" {ty_ovar 1} {ty_ovar 0})) "sigma")))))
+        ----------------------------------------------- ("typerec func") (* trec-fn on page 135 *)
+        #"typerec" (#"->" "t1" "t2") "sigma" "e1" "e2" "e3"
+        = #"app" (@"@" @("A" := {A_var}) (#"app" (#"@" "e3" "t1") (#"typerec" "t1" "sigma" "e1" "e2" "e3")) "t2") (#"typerec" "t2" "sigma" "e1" "e2" "e3")
+        : #"exp" "D" "G" (#"ty_subst" (#"ty_snoc" #"ty_id" (#"->" "t1" "t2")) "sigma")                  
+    ];
+    [:= "D" : #"ty_env",
+        "G" : #"env" "D",
+        "G'" : #"env" "D",
+        "g" : #"sub" "D" "G'" "G",
+        "mu" : #"ty" "D",
+        "sigma" : #"ty" (#"ty_ext" "D"),
+        "e1" : #"exp" "D" "G" (#"ty_subst" (#"ty_snoc" #"ty_id" #"*") "sigma"),
+        "e2" : #"exp" "D" "G" (#"ty_subst" (#"ty_snoc" #"ty_id" #"bool") "sigma"),
+        "e3" : #"exp" "D" "G" (#"All" (#"->" "sigma" (#"All" (#"->" (#"ty_subst" (#"ty_snoc" {ty_wkn_n 2} {ty_ovar 0}) "sigma") (#"ty_subst" (#"ty_snoc" {ty_wkn_n 2} (#"->" {ty_ovar 1} {ty_ovar 0})) "sigma")))))
+        ----------------------------------------------- ("exp_subst typerec")
+        #"exp_subst" "g" (#"typerec" "mu" "sigma" "e1" "e2" "e3")
+        = #"typerec" "mu" "sigma" (#"exp_subst" "g" "e1") (#"exp_subst" "g" "e2") (#"exp_subst" "g" "e3")
+        : #"exp" "D" "G'" (#"ty_subst" (#"ty_snoc" #"ty_id" "mu") "sigma")
+    ];
+    [:= "D" : #"ty_env",
+        "D'" : #"ty_env",
+        "G" : #"env" "D",
+        "g" : #"ty_sub" "D'" "D",
+        "mu" : #"ty" "D",
+        "sigma" : #"ty" (#"ty_ext" "D"),
+        "e1" : #"exp" "D" "G" (#"ty_subst" (#"ty_snoc" #"ty_id" #"*") "sigma"),
+        "e2" : #"exp" "D" "G" (#"ty_subst" (#"ty_snoc" #"ty_id" #"bool") "sigma"),
+        "e3" : #"exp" "D" "G" (#"All" (#"->" "sigma" (#"All" (#"->" (#"ty_subst" (#"ty_snoc" {ty_wkn_n 2} {ty_ovar 0}) "sigma") (#"ty_subst" (#"ty_snoc" {ty_wkn_n 2} (#"->" {ty_ovar 1} {ty_ovar 0})) "sigma")))))
+        ----------------------------------------------- ("ty_subst typerec")
+        #"exp_ty_subst" "g" (#"typerec" "mu" "sigma" "e1" "e2" "e3")
+        = #"typerec" (#"ty_subst" "g" "mu") (#"ty_subst" (#"ty_snoc" (#"ty_cmp" #"ty_wkn" "g") #"ty_hd") "sigma") (#"exp_ty_subst" "g" "e1") (#"exp_ty_subst" "g" "e2") (#"exp_ty_subst" "g" "e3")
+        : #"exp" "D'" (#"env_ty_subst" "g" "G") (#"ty_subst" "g" (#"ty_subst" (#"ty_snoc" #"ty_id" "mu") "sigma"))
+    ]
+  ]}.
+
+Derive type_casing
+  SuchThat (elab_lang_ext (
+                stlc_ty_subst ++
+                  typed_bool_ty_subst ++ 
+                  usubst_ty_subst ++
+                  typed_bool_parameterized ++
+                  stlc_parameterized ++
+                  usubst_parameterized ++
+                  poly ++ (* needed for #"All" *)
+                  (* below are the things needed for polymorphic languages *)
+                  exp_param_substs ++
+                  exp_ty_subst ++
+                  val_param_substs ++
+                  val_ty_subst ++
+                  env_ty_subst ++
+                  ty_subst_lang ++
+                  exp_parameterized ++ val_parameterized ++ ty_env_lang
+              ) 
+                type_casing_def type_casing)
+        As type_casing_wf.
+Proof. 
+  auto_elab. (* 6:20 *)
+Qed. (* ~0:30 *)
+#[export] Hint Resolve type_casing_wf : elab_pfs.
+
+(* 
+TODO:
+- simple to poly compiler
+  - convoy for simple to poly compiler
+  - remaining langs parameterized (ultc_bool, mif, uif, boolhuh)
+- poly to poly compiler
+  - parameterize boundaries (* STARTED, not done *)
+  - convoy for poly to poly compiler
+*)
+
+
+(* The actual multilanguages *)
+(* QUESTION: if the target language has polymorphism, can we still define a shared fragment? *)
+(* correct. need to redo this to basically just insert empty environment anywhere *)
+(* with Dustin notation, so long as differing metavars are just implicit, then writing no rules will work. worst you will have to do is the A variable stuff *)
+
+Definition utlc_parameterized := 
+    let ps := (elab_param "D" (utlc ++ usubst ++ exp_ret ++ exp_subst_base
+                                 ++ value_subst)
+               [("sub", Some 2);
+                ("ty", Some 0);
+                ("env", Some 0);
+                ("val",Some 2);
+                ("exp",Some 2)]) in
+  parameterize_lang "D" {{s #"ty_env"}}
+    ps utlc.
+
+Local Definition evp'_utlc : lang := 
+    let ps := (elab_param "D" (utlc ++ usubst ++ exp_ret ++ exp_subst_base
+                                 ++ value_subst)
+               [("sub", Some 2);
+                ("ty", Some 0);
+                ("env", Some 0);
+                ("val",Some 2);
+                ("exp",Some 2)]) in
+  parameterize_lang "D" {{s #"ty_env"}}
+    ps (usubst ++ exp_ret ++ exp_subst_base ++ value_subst).
+
+Lemma utlc_parameterized_wf
+  : wf_lang_ext ((usubst_parameterized ++ exp_parameterized ++ val_parameterized) ++ ty_env_lang)
+      utlc_parameterized.
+Proof. 
+  replace (usubst_parameterized ++ exp_parameterized ++ val_parameterized) with evp'_utlc.
+  - eapply parameterize_lang_preserving_ext;
+    try typeclasses eauto;
+    [repeat t';  constructor (*TODO: include in t'*)
+    | now prove_from_known_elabs..
+    | vm_compute; exact I].
+  - cbv; reflexivity. 
+Qed. 
+#[export] Hint Resolve utlc_parameterized_wf : elab_pfs.
+
+Definition untyped_bool_parameterized := 
+    let ps := (elab_param "D" (untyped_bool ++ usubst ++ exp_ret ++ exp_subst_base
+                                 ++ value_subst)
+               [("sub", Some 2);
+                ("ty", Some 0);
+                ("env", Some 0);
+                ("val",Some 2);
+                ("exp",Some 2)]) in
+  parameterize_lang "D" {{s #"ty_env"}}
+    ps untyped_bool.
+
+Local Definition evp'_untyped_bool : lang := 
+    let ps := (elab_param "D" (untyped_bool ++ usubst ++ exp_ret ++ exp_subst_base
+                                 ++ value_subst)
+               [("sub", Some 2);
+                ("ty", Some 0);
+                ("env", Some 0);
+                ("val",Some 2);
+                ("exp",Some 2)]) in
+  parameterize_lang "D" {{s #"ty_env"}}
+    ps (usubst ++ exp_ret ++ exp_subst_base ++ value_subst).
+
+Lemma untyped_bool_parameterized_wf
+  : wf_lang_ext ((usubst_parameterized ++ exp_parameterized ++ val_parameterized) ++ ty_env_lang)
+      untyped_bool_parameterized.
+Proof. 
+  replace (usubst_parameterized ++ exp_parameterized ++ val_parameterized) with evp'_untyped_bool.
+  - eapply parameterize_lang_preserving_ext;
+    try typeclasses eauto;
+    [repeat t';  constructor (*TODO: include in t'*)
+    | now prove_from_known_elabs..
+    | vm_compute; exact I].
+  - cbv; reflexivity. 
+Qed. 
+#[export] Hint Resolve utlc_parameterized_wf : elab_pfs.
+
+Definition utlc_bool_parameterized := 
+    let ps := (elab_param "D" (utlc_bool ++ untyped_bool ++ utlc ++ usubst ++ exp_ret ++ exp_subst_base ++ value_subst)
+               [("sub", Some 2);
+                ("ty", Some 0);
+                ("env", Some 0);
+                ("val",Some 2);
+                ("exp",Some 2)]) in
+  parameterize_lang "D" {{s #"ty_env"}}
+    ps utlc_bool.
+
+Local Definition evp'_utlc_bool : lang := 
+    let ps := (elab_param "D" (utlc_bool ++ untyped_bool ++ utlc ++ usubst ++ exp_ret ++ exp_subst_base ++ value_subst)
+               [("sub", Some 2);
+                ("ty", Some 0);
+                ("env", Some 0);
+                ("val",Some 2);
+                ("exp",Some 2)]) in
+  parameterize_lang "D" {{s #"ty_env"}}
+    ps (untyped_bool ++ utlc ++ usubst ++ exp_ret ++ exp_subst_base ++ value_subst).
+
+Lemma utlc_bool_parameterized_wf
+  : wf_lang_ext ((untyped_bool_parameterized ++ utlc_parameterized ++ usubst_parameterized ++ exp_parameterized ++ val_parameterized) ++ ty_env_lang)
+      utlc_bool_parameterized.
+Proof. 
+  replace (untyped_bool_parameterized ++ utlc_parameterized ++ usubst_parameterized ++ exp_parameterized ++ val_parameterized) with evp'_utlc_bool.
+  - eapply parameterize_lang_preserving_ext;
+    try typeclasses eauto;
+    [repeat t';  constructor (*TODO: include in t'*)
+    | now prove_from_known_elabs..
+    | vm_compute; exact I].
+  - cbv; reflexivity. 
+Qed. 
+#[export] Hint Resolve utlc_bool_parameterized_wf : elab_pfs.
+
+Definition boolhuh_parameterized := 
+    let ps := (elab_param "D" (boolhuh ++ untyped_bool ++ utlc ++ usubst ++ exp_ret ++ exp_subst_base ++ value_subst)
+               [("sub", Some 2);
+                ("ty", Some 0);
+                ("env", Some 0);
+                ("val",Some 2);
+                ("exp",Some 2)]) in
+  parameterize_lang "D" {{s #"ty_env"}}
+    ps boolhuh.
+
+Local Definition evp'_boolhuh : lang := 
+    let ps := (elab_param "D" (boolhuh ++ untyped_bool ++ utlc ++ usubst ++ exp_ret ++ exp_subst_base ++ value_subst)
+               [("sub", Some 2);
+                ("ty", Some 0);
+                ("env", Some 0);
+                ("val",Some 2);
+                ("exp",Some 2)]) in
+  parameterize_lang "D" {{s #"ty_env"}}
+    ps (untyped_bool ++ utlc ++ usubst ++ exp_ret ++ exp_subst_base ++ value_subst).
+
+Lemma boolhuh_parameterized_wf
+  : wf_lang_ext ((untyped_bool_parameterized ++ utlc_parameterized ++ usubst_parameterized ++ exp_parameterized ++ val_parameterized) ++ ty_env_lang)
+      boolhuh_parameterized.
+Proof. 
+  replace (untyped_bool_parameterized ++ utlc_parameterized ++ usubst_parameterized ++ exp_parameterized ++ val_parameterized) with evp'_boolhuh.
+  - eapply parameterize_lang_preserving_ext;
+    try typeclasses eauto;
+    [repeat t';  constructor (*TODO: include in t'*)
+    | now prove_from_known_elabs..
+    | vm_compute; exact I].
+  - cbv; reflexivity. 
+Qed. 
+#[export] Hint Resolve boolhuh_parameterized_wf : elab_pfs.
+
+Definition simple_shared_fragment :=
+  boolhuh ++ 
+    utlc_bool ++ 
+    utlc ++ 
+    untyped_bool ++ 
+    usubst ++ 
+    typed_bool ++ 
+    stlc ++ 
+    exp_subst ++ 
+    value_subst. 
+Hint Unfold simple_shared_fragment : auto_elab.
+
+Definition polymorphic_shared_fragment :=
+    boolhuh_parameterized ++ 
+    utlc_bool_parameterized ++ 
+    utlc_parameterized ++
+    (* stlc_ty_subst ++ (* ty_subst lang *)
+    typed_bool_ty_subst ++ (* ty_subst lang *)
+    usubst_ty_subst ++ (* ty_subst lang *) *)
+    untyped_bool_parameterized ++ 
+    usubst_parameterized ++ 
+    typed_bool_parameterized ++ 
+    stlc_parameterized ++
+    (* all polymorphic langs stuff *)
+    exp_param_substs ++
+    exp_ty_subst ++
+    val_param_substs ++
+    val_ty_subst ++
+    env_ty_subst ++
+    ty_subst_lang ++
+    exp_parameterized ++ val_parameterized ++ ty_env_lang.
+Hint Unfold polymorphic_shared_fragment : auto_elab.
+
+Local Notation compiler := (compiler string).
+
+Compute value_subst. Locate exp_subst.  
+
+Definition shared_fragment_compiler_def : compiler :=
+  match # from simple_shared_fragment with
+  | {{s#"ty"}} => {{s #"ty" #"ty_emp"}}
+  | {{s#"env"}} => {{s #"env" #"ty_emp"}}
+  | {{s#"sub" "G" "G'"}} => {{s #"sub" #"ty_emp" "G" "G'"}}
+  | {{e#"id" "G"}} => {{e @"id" @("D" := #"ty_emp")}}
+  | {{e#"cmp" "G1" "G2" "G3" "f" "g"}} => {{e @"cmp" @("D" := #"ty_emp") "f" "g"}}
+  | {{s#"val" "G" "A"}} => {{s #"val" #"ty_emp" "G" "A"}}
+  | {{e#"val_subst" "G" "G'" "g" "A" "v"}} => {{e @"val_subst" @("D" := #"ty_emp") "g" "v"}}
+  | {{e#"emp"}} => {{e @"emp" @("D" := #"ty_emp")}}
+  | {{e#"forget" "G"}} => {{e @"forget" @("D" := #"ty_emp")}}
+  | {{e#"ext" "G" "A"}} => {{e @"ext" @("D" := #"ty_emp") "G" "A"}}
+  | {{e#"snoc" "G" "G'" "g" "A" "v"}} => {{e @"snoc" @("D" := #"ty_emp") "g" "v"}}
+  | {{e#"wkn" "G" "A"}} => {{e @"wkn" @("D" := #"ty_emp")}}
+  | {{e#"hd" "G" "A"}} => {{e @"hd" @("D" := #"ty_emp")}}
+  | {{s#"exp" "G" "A"}} => {{s #"exp" #"ty_emp" "G" "A"}}
+  | {{e#"exp_subst" "G" "G'" "g" "A" "e"}} => {{e @"exp_subst" @("D" := #"ty_emp") "g" "e"}}
+  | {{e#"ret" "G" "A" "v"}} => {{e @"ret" @("D" := #"ty_emp") "v"}}
+  | {{e#"->" "t" "t'"}} => {{e @"->" @("D" := #"ty_emp") "t" "t'"}}
+  | {{e#"lambda" "G" "A" "B" "e"}} => {{e @"lambda" @("D" := #"ty_emp") "A" "e"}}
+  | {{e#"app" "G" "A" "B" "e" "e'"}} => {{e @"app" @("D" := #"ty_emp") "e" "e'"}}
+  | {{e#"bool"}} => {{e @"bool" @("D" := #"ty_emp")}}
+  | {{e#"T" "G"}} => {{e @"T" @("D" := #"ty_emp")}}
+  | {{e#"F" "G"}} => {{e @"F" @("D" := #"ty_emp")}}
+  | {{e#"if" "G" "A" "cond" "e2" "e3"}} => {{e @"if" @("D" := #"ty_emp") "cond" "e2" "e3"}}
+  | {{e#"*"}} => {{e @"*" @("D" := #"ty_emp")}}
+  | {{e#"Error" "G" "t"}} => {{e @"Error" @("D" := #"ty_emp") "t"}}
+  | {{e#"uT" "G"}} => {{e @"uT" @("D" := #"ty_emp")}}
+  | {{e#"uF" "G"}} => {{e @"uF" @("D" := #"ty_emp")}}
+  | {{e#"ulambda" "G" "e"}} => {{e @"ulambda" @("D" := #"ty_emp") "e"}}
+  | {{e#"uapp" "G" "e" "e'"}} => {{e @"uapp" @("D" := #"ty_emp") "e" "e'"}}
+  | {{e#"bool?" "G" "e"}} => {{e @"bool?" @("D" := #"ty_emp") "e"}}
+  end.
+
+Compute shared_fragment_compiler_def. 
+
+Axiom todo : wf_lang polymorphic_shared_fragment.
+
+Derive shared_fragment_compiler 
+        SuchThat (elab_preserving_compiler 
+                    []
+                    polymorphic_shared_fragment
+                    shared_fragment_compiler_def
+                    shared_fragment_compiler
+                    simple_shared_fragment) 
+        As shared_fragment_compiler_preserving. 
+Proof.
+  assert (wf_lang polymorphic_shared_fragment) by apply todo.
+  auto_elab_compiler.
+Qed.
+Hint Resolve shared_fragment_compiler_preserving : auto_elab. 
+
+Definition mif_parameterized := 
+    let ps := (elab_param "D" (mif ++ untyped_bool ++ utlc ++ usubst ++ exp_ret ++ exp_subst_base ++ value_subst)
+               [("sub", Some 2);
+                ("ty", Some 0);
+                ("env", Some 0);
+                ("val",Some 2);
+                ("exp",Some 2)]) in
+  parameterize_lang "D" {{s #"ty_env"}}
+    ps mif.
+
+Local Definition evp'_mif : lang := 
+    let ps := (elab_param "D" (mif ++ untyped_bool ++ utlc ++ usubst ++ exp_ret ++ exp_subst_base ++ value_subst)
+               [("sub", Some 2);
+                ("ty", Some 0);
+                ("env", Some 0);
+                ("val",Some 2);
+                ("exp",Some 2)]) in
+  parameterize_lang "D" {{s #"ty_env"}}
+    ps (untyped_bool ++ utlc ++ usubst ++ exp_ret ++ exp_subst_base ++ value_subst).
+
+Lemma mif_parameterized_wf
+  : wf_lang_ext ((untyped_bool_parameterized ++ utlc_parameterized ++ usubst_parameterized ++ exp_parameterized ++ val_parameterized) ++ ty_env_lang)
+      mif_parameterized.
+Proof. 
+  replace (untyped_bool_parameterized ++ utlc_parameterized ++ usubst_parameterized ++ exp_parameterized ++ val_parameterized) with evp'_mif.
+  - eapply parameterize_lang_preserving_ext;
+    try typeclasses eauto;
+    [repeat t';  constructor (*TODO: include in t'*)
+    | now prove_from_known_elabs..
+    | vm_compute; exact I].
+  - cbv; reflexivity. 
+Qed. 
+#[export] Hint Resolve mif_parameterized_wf : elab_pfs.
+
+Definition source_multilanguage := 
+            boundaries ++ uif ++ simple_shared_fragment.
+Hint Unfold source_multilanguage : auto_elab. 
+
+Definition target_multilanguage :=
+            type_casing ++ mif_parameterized ++ polymorphic_shared_fragment.
+Hint Unfold target_multilanguage : auto_elab.
+
+Compute mif_parameterized.
+Compute value_subst. 
+
+(*
+Definition ttd_fun t1 (x : t1 -> dyn) t2 (y : t2 -> dyn) : (t1 -> t2) -> dyn :=
+  fun input =>
+    ufun z =>
+    y (input (dtt t1 z))
+.
+Definition ttd t : t -> dyn :=
+  match t with
+  | dyn => fun x => x
+  | bool => fun x =>  if x then utrue else ufalse
+  | t1 -> t2 => fun t1 (x : t1 -> dyn) t2 (y : t2 -> dyn) => fun input =>
+    ufun z =>
+      y (input (dtt t1 z))
+  end.
+
+Definition dtt t : dyn -> t :=
+  match t with
+  | dyn => fun x => x
+  | bool => fun x =>  mif x then true else false
+  | t1 -> t2 => fun t1 (x : dyn -> t1) t2 (y : dyn -> t2) => ufun input =>
+    fun z =>
+      y (input (ttd t1 z))
+  end.
+
+Definition boundaries t : (t -> dyn) * (dyn -> t) :=
+  match t with
+  | dyn => (fun x => x, fun x => x)
+  | bool => (fun x =>  if x then utrue else ufalse, fun x =>  mif x then true else false)
+  | t1 -> t2 => fun t1 (x : (t1 -> dyn) * (dyn -> t1)) t2 (y : (t2 -> dyn) * (dyn -> t2)) =>
+                  (
+                    fun input =>
+    ufun z =>
+      (fst y) (input ((snd x) z))
+                    ,
+                    ufun input =>
+    fun z =>
+      (snd y) (input ((fst x) z))
+                    )
+  end.
+*)
+
+
+(* simple to poly compiler *)
+Definition multilang_compiler_def : compiler :=
+    match # from (boundaries ++ uif) with
+    | {{e #"uif" "G" "c" "thn" "els"}} => {{e @"mif" @("D" := #"ty_emp") "c" "thn" "els" }}
+    | {{e #"dtt" "G" "A" "e"}} => {{e (* NOT convoy *)
+                                    #"typerec" "A" #"ty_hd"
+                                    "e" 
+                                    (#"mif" "e" (#"ret" #"T") (#"ret" #"F")) 
+                                    (#"ret" (#"lambda" "A" (#"dtt" "C" (#"uapp" (#"ret" (#"val_subst" #"wkn" "v")) (#"ttd" "B" (#"ret" #"hd")))))) 
+                                    }}
+    | {{e #"ttd" "G" "A" "e"}} => {{e (* NEED convoy *)
+                                      #"typerec" "A" #"ty_hd"
+                                      (#"lambda" "A" #"hd")
+                                      (#"lambda" "A" (#"if" #"hd" (#"ret" #"uT") (#"ret" #"uF")))
+                                      (#"lambda" "A" (#"ret" (#"ulambda" (#"ttd" "C" (#"app" (#"ret" (#"val_subst" #"wkn" #"hd")) (#"dtt" "B" (#"ret" #"hd")))))))
+                                    "e"
+                                    }}
+    (* order of implicit vars is order of context vars *)
+    (* neeed to parameterize exp sort and val sort and ty sort so need three rules for that *)
+    end.
+
+Compute multilang_compiler_def. 
+
+(* in case needed, defined in Tools.Matches, Elab.ElabCompilers *)
+(* semantic properties are in SemanticsPreservingDefs.v *)
+
+(* Locate elab_preserving_compiler. 
+Locate auto_elab_compiler.  *)
+
+Derive multilang_compiler 
+        SuchThat (elab_preserving_compiler 
+                    shared_fragment_compiler
+                    target_multilanguage
+                    multilang_compiler_def
+                    multilang_compiler
+                    (boundaries ++ uif)
+                    ) 
+        As multilang_compiler_preserving. 
+Proof. 
+Abort. 
+
+
+
+
+
+
+
+
+Local Notation preserving_compiler_ext tgt cmp_pre cmp src := (* copied from Paramaterizer, 2523 *)
+(preserving_compiler_ext (tgt_Model:=core_model tgt) cmp_pre cmp src).
+
+Definition polymorphic_shared_fragment_compiler := id_compiler polymorphic_shared_fragment. 
+
+Lemma polymorphic_shared_fragment_identity_compiler_preserving : preserving_compiler_ext polymorphic_shared_fragment [] polymorphic_shared_fragment_compiler polymorphic_shared_fragment.
+Proof. Abort.
+(*
+    (* OLD TACTICS (for some reason this doesn't work now?) *)
+    unfold polymorphic_shared_fragment. 
+    apply id_compiler_preserving; prove_from_known_elabs. 
+    typeclasses eauto.
+Qed.
+Hint Resolve polymorphic_shared_fragment_identity_compiler_preserving : auto_elab.
+*)
 
 Definition boundaries_parameterized_def : lang :=
   {[l
@@ -496,283 +919,13 @@ Proof. Abort.
 (* #[export] Hint Resolve boundaries_parameterized_wf : elab_pfs. *)
 
 
-Fixpoint ty_wkn_n n :=
-  match n with
-  | 0 => {{e #"ty_id"}}
-  | 1 => {{e #"ty_wkn"}}
-  | S n' => {{e #"ty_cmp" #"ty_wkn" {ty_wkn_n n'} }}
-  end.
-
-Definition ty_ovar n :=
-  match n with 
-  | 0 => {{e #"ty_hd"}} (* bc ty_subst ty_id ty_hd is just ty_hd *)
-  | S _ => {{e #"ty_subst" {ty_wkn_n n} #"ty_hd" }}
-  end.  
-
-(* for reference, computation of all languages that type casing depends on, in reverse order of simplicity *)
-Compute ty_env_lang.
-Compute val_parameterized.
-Compute exp_parameterized.
-Compute ty_subst_lang. (* this is where ty_subst is defined *)
-Compute env_ty_subst.
-Compute val_ty_subst.
-Compute val_param_substs.
-Compute exp_ty_subst.
-Compute exp_param_substs.
-Compute poly.
-Compute usubst_parameterized.
-Compute stlc_parameterized.
-Compute typed_bool_parameterized. 
-Compute exp_subst_def. 
-Compute ty_subst_lang. 
-
-(* other old stuff *)
-Locate ty_subst_lang. 
-Compute ty_subst_def. (* I think this has an example of type substitution, which is the rule you're mising in the type casing language *)
-
-Definition A_var := {{e #"ty_subst" (#"ty_snoc" (#"ty_cmp" #"ty_wkn" (#"ty_snoc" #"ty_id" "t1")) #"ty_hd") (#"->" (#"ty_subst" (#"ty_snoc" {ty_wkn_n 2} {ty_ovar 0}) "sigma") (#"ty_subst" (#"ty_snoc" {ty_wkn_n 2} (#"->" {ty_ovar 1} {ty_ovar 0})) "sigma")) }}.
-
-(* trying to fix the type issue: manual computation of the expected type *)
-Definition g := {{e #"ty_snoc" #"ty_id" "t2" }}.
-Definition h := {{e #"ty_snoc" (#"ty_cmp" #"ty_wkn" (#"ty_snoc" #"ty_id" "t1")) #"ty_hd" }}.
-Definition final_Sigma := {{e #"ty_subst" (#"ty_snoc" {ty_wkn_n 2} (#"->" {ty_ovar 1} {ty_ovar 0})) "sigma" }}.
-Definition desired_type := {{e #"ty_subst" (#"ty_cmp" {g} {h}) {final_Sigma} }}.
-
-Definition type_casing_def : lang :=
-  {[l
-    [:| "D" : #"ty_env",
-        "G" : #"env" "D",
-        "mu" : #"ty" "D", (* is mu *)
-        "sigma" : #"ty" (#"ty_ext" "D"), (* this is sigma. it's a variable? I think? *)
-        "e1" : #"exp" "D" "G" (#"ty_subst" (#"ty_snoc" #"ty_id" #"*") "sigma"), (* substitute identity type for all except the last (which is A), which we change to star *)
-        "e2" : #"exp" "D" "G" (#"ty_subst" (#"ty_snoc" #"ty_id" #"bool") "sigma"),
-        "e3" : #"exp" "D" "G" (#"All" (#"->" "sigma" (#"All" (#"->" (#"ty_subst" (#"ty_snoc" {ty_wkn_n 2} {ty_ovar 0}) "sigma") (#"ty_subst" (#"ty_snoc" {ty_wkn_n 2} (#"->" {ty_ovar 1} {ty_ovar 0})) "sigma"))))) (* look at arrow case in 134 *)
-        -----------------------------------------------
-        #"typerec" "mu" "sigma" "e1" "e2" "e3"
-        : #"exp" "D" "G" (#"ty_subst" (#"ty_snoc" #"ty_id" "mu") "sigma") (* verbose way of writing the [u/t]sigma in the rule on 134 *)
-    ];
-    [:= "D" : #"ty_env",
-        "G" : #"env" "D",
-        "sigma" : #"ty" (#"ty_ext" "D"),
-        "e1" : #"exp" "D" "G" (#"ty_subst" (#"ty_snoc" #"ty_id" #"*") "sigma"),
-        "e2" : #"exp" "D" "G" (#"ty_subst" (#"ty_snoc" #"ty_id" #"bool") "sigma"),
-        "e3" : #"exp" "D" "G" (#"All" (#"->" "sigma" (#"All" (#"->" (#"ty_subst" (#"ty_snoc" {ty_wkn_n 2} {ty_ovar 0}) "sigma") (#"ty_subst" (#"ty_snoc" {ty_wkn_n 2} (#"->" {ty_ovar 1} {ty_ovar 0})) "sigma")))))
-        ----------------------------------------------- ("typerec star")
-        #"typerec" #"*" "sigma" "e1" "e2" "e3"  
-        = "e1" : #"exp" "D" "G" (#"ty_subst" (#"ty_snoc" #"ty_id" #"*") "sigma")
-    ];
-    [:= "D" : #"ty_env",
-        "G" : #"env" "D",
-        "sigma" : #"ty" (#"ty_ext" "D"),
-        "e1" : #"exp" "D" "G" (#"ty_subst" (#"ty_snoc" #"ty_id" #"*") "sigma"),
-        "e2" : #"exp" "D" "G" (#"ty_subst" (#"ty_snoc" #"ty_id" #"bool") "sigma"),
-        "e3" : #"exp" "D" "G" (#"All" (#"->" "sigma" (#"All" (#"->" (#"ty_subst" (#"ty_snoc" {ty_wkn_n 2} {ty_ovar 0}) "sigma") (#"ty_subst" (#"ty_snoc" {ty_wkn_n 2} (#"->" {ty_ovar 1} {ty_ovar 0})) "sigma")))))
-        ----------------------------------------------- ("typerec bool")
-        #"typerec" #"bool" "sigma" "e1" "e2" "e3"  
-        = "e2" : #"exp" "D" "G" (#"ty_subst" (#"ty_snoc" #"ty_id" #"bool") "sigma")
-    ];
-    [:= "D" : #"ty_env",
-        "G" : #"env" "D",
-        "sigma" : #"ty" (#"ty_ext" "D"),
-        "t1" : #"ty" "D",
-        "t2" : #"ty" "D",
-        "e1" : #"exp" "D" "G" (#"ty_subst" (#"ty_snoc" #"ty_id" #"*") "sigma"),
-        "e2" : #"exp" "D" "G" (#"ty_subst" (#"ty_snoc" #"ty_id" #"bool") "sigma"),
-        "e3" : #"exp" "D" "G" (#"All" (#"->" "sigma" (#"All" (#"->" (#"ty_subst" (#"ty_snoc" {ty_wkn_n 2} {ty_ovar 0}) "sigma") (#"ty_subst" (#"ty_snoc" {ty_wkn_n 2} (#"->" {ty_ovar 1} {ty_ovar 0})) "sigma")))))
-        ----------------------------------------------- ("typerec func") (* trec-fn on page 135 *)
-        #"typerec" (#"->" "t1" "t2") "sigma" "e1" "e2" "e3"
-        = #"app" (@"@" @("A" := {A_var}) (#"app" (#"@" "e3" "t1") (#"typerec" "t1" "sigma" "e1" "e2" "e3")) "t2") (#"typerec" "t2" "sigma" "e1" "e2" "e3")
-        (* : #"exp" "D" "G" {desired_type} *)
-        : #"exp" "D" "G" (#"ty_subst" (#"ty_snoc" #"ty_id" (#"->" "t1" "t2")) "sigma")                  
-    ];
-    [:= "D" : #"ty_env",
-        "G" : #"env" "D",
-        "G'" : #"env" "D",
-        "g" : #"sub" "D" "G'" "G",
-        "mu" : #"ty" "D",
-        "sigma" : #"ty" (#"ty_ext" "D"),
-        "e1" : #"exp" "D" "G" (#"ty_subst" (#"ty_snoc" #"ty_id" #"*") "sigma"),
-        "e2" : #"exp" "D" "G" (#"ty_subst" (#"ty_snoc" #"ty_id" #"bool") "sigma"),
-        "e3" : #"exp" "D" "G" (#"All" (#"->" "sigma" (#"All" (#"->" (#"ty_subst" (#"ty_snoc" {ty_wkn_n 2} {ty_ovar 0}) "sigma") (#"ty_subst" (#"ty_snoc" {ty_wkn_n 2} (#"->" {ty_ovar 1} {ty_ovar 0})) "sigma")))))
-        ----------------------------------------------- ("exp_subst typerec")
-        #"exp_subst" "g" (#"typerec" "mu" "sigma" "e1" "e2" "e3")
-        = #"typerec" "mu" "sigma" (#"exp_subst" "g" "e1") (#"exp_subst" "g" "e2") (#"exp_subst" "g" "e3")
-        : #"exp" "D" "G'" (#"ty_subst" (#"ty_snoc" #"ty_id" "mu") "sigma")
-    ];
-    [:= "D" : #"ty_env",
-        "D'" : #"ty_env",
-        "G" : #"env" "D",
-        "g" : #"ty_sub" "D'" "D",
-        "mu" : #"ty" "D",
-        "sigma" : #"ty" (#"ty_ext" "D"),
-        "e1" : #"exp" "D" "G" (#"ty_subst" (#"ty_snoc" #"ty_id" #"*") "sigma"),
-        "e2" : #"exp" "D" "G" (#"ty_subst" (#"ty_snoc" #"ty_id" #"bool") "sigma"),
-        "e3" : #"exp" "D" "G" (#"All" (#"->" "sigma" (#"All" (#"->" (#"ty_subst" (#"ty_snoc" {ty_wkn_n 2} {ty_ovar 0}) "sigma") (#"ty_subst" (#"ty_snoc" {ty_wkn_n 2} (#"->" {ty_ovar 1} {ty_ovar 0})) "sigma")))))
-        ----------------------------------------------- ("ty_subst typerec")
-        #"exp_ty_subst" "g" (#"typerec" "mu" "sigma" "e1" "e2" "e3")
-        = #"typerec" (#"ty_subst" "g" "mu") (#"ty_subst" (#"ty_snoc" (#"ty_cmp" #"ty_wkn" "g") #"ty_hd") "sigma") (#"exp_ty_subst" "g" "e1") (#"exp_ty_subst" "g" "e2") (#"exp_ty_subst" "g" "e3")
-        : #"exp" "D'" (#"env_ty_subst" "g" "G") (#"ty_subst" "g" (#"ty_subst" (#"ty_snoc" #"ty_id" "mu") "sigma"))
-    ]
-  ]}.
-
-(* Compute type_casing_def.  *)
-Derive type_casing
-        SuchThat (elab_lang_ext (
-                                stlc_poly ++ (* has the subst-arrow distribution rule *)
-                                typed_bool_parameterized ++
-                                typed_bool_parameterized' ++ 
-                                stlc_parameterized ++ (* still need it for definitions *)  
-                                usubst_parameterized ++
-                                usubst_parameterized' ++
-                                poly ++ (* needed for #"All" *)
-                                (* below are the things needed for polymorphic languages *)
-                                exp_param_substs ++
-                                exp_ty_subst ++
-                                val_param_substs ++
-                                val_ty_subst ++
-                                env_ty_subst ++
-                                ty_subst_lang ++
-                                exp_parameterized ++ val_parameterized ++ ty_env_lang
-                                ) 
-                type_casing_def type_casing)
-        As type_casing_wf.
-Proof. 
-  auto_elab. (* 6:20 *)
-Qed. 
-#[export] Hint Resolve type_casing_wf : elab_pfs.
-
-
-(* The actual multilanguages *)
-Definition shared_fragment := 
-            boolhuh ++ (* think abt why can't compile s*)
-            utlc_bool ++ utlc ++ untyped_bool ++ usubst ++
-            typed_bool ++ stlc ++
-            exp_subst ++ value_subst.
-Hint Unfold shared_fragment : auto_elab. 
-
-Local Notation preserving_compiler_ext tgt cmp_pre cmp src := (* copied from Paramaterizer, 2523 *)
-(preserving_compiler_ext (tgt_Model:=core_model tgt) cmp_pre cmp src).
-
-Definition shared_fragment_compiler := id_compiler shared_fragment. 
-
-Lemma shared_fragment_compiles : preserving_compiler_ext shared_fragment [] shared_fragment_compiler shared_fragment.
-Proof. 
-    unfold shared_fragment. 
-    apply id_compiler_preserving; prove_from_known_elabs. 
-    typeclasses eauto. 
-Qed. 
-Hint Resolve shared_fragment_compiles : auto_elab. 
-
-Definition source_multilanguage := 
-            boundaries ++ uif ++ shared_fragment.
-Hint Unfold source_multilanguage : auto_elab. 
-
-Definition target_multilanguage :=
-            type_casing ++ mif ++ shared_fragment.
-Hint Unfold target_multilanguage : auto_elab. 
-
-(* Print boolhuh.  *)
-(* here you can see implicit arguments *)
-
-(* the compiler *)
-Local Notation compiler := (compiler string). 
-Definition multilang_compiler_def : compiler :=
-    match # from (boundaries ++ uif) with
-    | {{e #"uif" "G" "c" "thn" "els"}} => {{e #"mif" "c" "thn" "els" }}
-    | {{e #"dtt" "G" "C" "e"}} => {{e #"type case" "C" (* diff from A below. TAKE CARE OF A AND B *)
-                                    "e" 
-                                    (#"mif" "e" (#"ret" #"T") (#"ret" #"F")) 
-                                    (* (#"Error" "C") *)
-                                    (#"ret" (#"lambda" "A" (#"dtt" "B" (#"uapp" (#"ret" (#"val_subst" #"wkn" "v")) (#"ttd" "A" (#"ret" #"hd")))))) 
-                                    }}
-    | {{e #"ttd" "G" "C" "e"}} => {{e #"type case" "C"  (* rewrite with convoy pattern focus on bool *)
-                                    "e"
-                                    (#"if" "e" (#"ret" #"uT") (#"ret" #"uF")) 
-                                    (#"Error" "C")
-                                    (* (#"ret" (#"ulambda" (#"ttd" "B" (#"app" (#"ret" (#"val_subst" #"wkn" "v")) (#"dtt" "A" (#"ret" #"hd"))))))  *)
-                                    }}
-    (* order of implicit vars is order of context vars *)
-    (* neeed to parameterize exp sort and val sort and ty sort so need three rules for that *)
-    end. 
-
-(* in case needed, defined in Tools.Matches, Elab.ElabCompilers *)
-(* semantic properties are in SemanticsPreservingDefs.v *)
-
-(* Locate elab_preserving_compiler. 
-Locate auto_elab_compiler.  *)
-
-Derive multilang_compiler 
-        SuchThat (elab_preserving_compiler 
-                    shared_fragment_compiler
-                    target_multilanguage
-                    multilang_compiler_def
-                    multilang_compiler
-                    (boundaries ++ uif)
-                    ) 
-        As multilang_compiler_preserving. 
-Proof. unfold low_level_multilanguage. 
-        unfold shared_fragment. 
-        unfold shared_fragment_compiler. 
-        auto_elab_compiler. 
 
 
 
-    (****** BEGIN In STUFF *)
-        cleanup_elab_after setup_elab_compiler.
-        1-3: shelve. 
 
-        - repeat ([> repeat Matches.t;
-           cleanup_elab_after try (try decompose_sort_eq; solve [ by_reduction ]) |..]).
-        - repeat ([> repeat Matches.t;
-           cleanup_elab_after try (try decompose_sort_eq; solve [ by_reduction ]) |..]).
-        - repeat ([> repeat Matches.t;
-           cleanup_elab_after try (try decompose_sort_eq; solve [ by_reduction ]) |..]).
-        - repeat ([> repeat Matches.t;
-           cleanup_elab_after try (try decompose_sort_eq; solve [ by_reduction ]) |..]).
-        - repeat ([> repeat Matches.t;
-           cleanup_elab_after try (try decompose_sort_eq; solve [ by_reduction ]) |..]).
-        - repeat ([> repeat Matches.t;
-           cleanup_elab_after try (try decompose_sort_eq; solve [ by_reduction ]) |..]).
-        - cbv [map combine fst]. 
-            (* cbv with brackets does _only_ those things. with the minus it does all but those htings. *)
 
-        (* cbn_elab_goal. *)
 
-        lazymatch goal with
-        | |- elab_term ?l ?ctx ?e ?ee ?t =>
-        let ctx' := eval cbv-[ann_cons annotation] in ctx in
-        let e' := eval cbv-[ann_cons annotation] in e in
-        let ee' := eval cbv-[ann_cons annotation] in ee in
-        let t' := eval cbv-[ann_cons annotation] in t in
-        change_no_check (elab_term l ctx' e' ee' t')
-        end. 
-        repeat t. 
-        
-        (****** END In STUFF *)
-        
-        
-        cbn_elab_goal. 
-        
-        (* convoy pattern *)
-        
-        auto_elab_compiler. 
-        1 : {
-            cbv -[In]. (* for in goals, this gives what you're trying to prove *)
-            Print auto_elab_compiler. 
-        }
-        3 : { admit. }
-        4 : { 
-                inversion h2l. 
-                Compute shared_fragment.  
-            }
-        (* is the name of a rule (replaces left to right)  *)
 
-        Locate shared_fragment. 
-        (* look at heap proofs, delete cleanup elab after *)
-        (* cleanup elab after are good for well formed terms *)
-        (* if you see elab_term, that means something is not done type inference *)
-        4 :{}
-Abort. 
 
 
 (* proof mirrors language proof *)
@@ -858,4 +1011,3 @@ Definition ttd_v {G : term} (x : term) (Ty : term) : Ty :=
                      end
   | {{e #"->" {A} {B} }} => {{e #"ulambda" {ttd_e {{e #"app" (#"val_subst" #"wkn" #"ret" {x}) {dtt_e {{e #"hd"}} A} }} B} }}
   end.  *)
-  Definition three := 3.
